Tengoku/EquationalTheories/Deps.lean
@@ -1,3 +1,4 @@
 import Tengoku.EquationalTheories.Deps.Equations
 import Tengoku.EquationalTheories.Deps.Magma
+import Tengoku.EquationalTheories.Deps.MemoFinOp
 import Tengoku.EquationalTheories.Deps.Superposition
